Another problem: How to make ptr2int to be total.
The current ptr2int has two cases
 ptr2int (Vint2ptr i) = i // the easy case
 ptr2int (Vptr b ofs) = ..?

The later case searchs the mapping from block-ofs to addresses, which
can be None if b does not exist. For example
  p = malloc ...;
  free p;
  i = ptrtoint p; // Here, the p is not valid, so we are stuck.

For the current proof (proving a value is not changed before and after a
malloc), this does not seem to be matter. Because,
1) if ptrtoint is legal before malloc, it should returns the same thing
after malloc, because malloc does not break existing blocks
2) if ptrtoint is None by pointing to a dead block, it should still
point to the dead block since malloc does not reuse any old blocks.

The rest reasoning is to show that a well-formed program cannot forge a
ptr to a blk-ofs out-of-thin-air, which could be a hard proof.

But, even the above idea works, it is not extensible to a practical
memory model that reuses memory.
 
One idea is to split Vint to be a normal Vint and a Vptrtoint b ofs;
keeping track free-ed blocks. But we still need to argue that a program
cannot 'create' a ptr w/o malloc --- pointing to a block that is not
form malloc. Secondly, this is not extensible to reallocating malloc
either, because at the case, a blk can be mapped to more than one
concrete addresses. 

The other idea is to let Vptr to be
  blk -> ofs -> addr -> val
here, the addr is its concrete addr.



git-svn-id: https://webdav.seas.upenn.edu/svn/sol/vol@2897 eef5ea85-cc2e-0410-bd84-0fae1f012da8

src/SoftBound/sb_trans.v
@@ -1693,11 +1693,216 @@ Global Opaque Mem.alloc.
       contradict H; auto.
 Qed.
 
+Definition veq Mem (v1 v2:val) : bool :=
+match v1, v2 with
+| Vundef, Vundef => true
+| Vundef, _ => false
+| _, Vundef => false
+| Vint wz1 i1, Vint wz2 i2 => zeq (Int.unsigned wz1 i1) (Int.unsigned wz2 i2)
+| Vint wz1 i1, Vfloat f2 => 
+    zeq (Int.unsigned wz1 i1) (Int.unsigned 31 (Floats.Float.intuoffloat f2))
+| Vfloat f1, Vint wz2 i2 => 
+    zeq (Int.unsigned 31 (Floats.Float.intuoffloat f1)) (Int.unsigned wz2 i2)
+| Vfloat f1, Vfloat f2 => match (Floats.Float.eq_dec f1 f2) with
+                          | left _ => true
+                          | right _ => false
+                          end
+| Vptr b1 o1, Vptr b2 o2 => eq_block b1 b2 && 
+                            zeq (Int.unsigned 31 o1) (Int.unsigned 31 o2)
+| Vinttoptr i1, Vinttoptr i2 => 
+    (* FIXME: Should we compare Vinttoptr and Vptr? *)
+    zeq (Int.unsigned 31 i1) (Int.unsigned 31 i2)
+| Vptr b1 o1, Vinttoptr i2 =>
+    match Mem.ptr2int Mem b1 0 with
+    | ret z => zeq (z + Int.signed 31 o1) (Int.unsigned 31 i2)
+    | merror => false
+    end
+| Vinttoptr i1, Vptr b2 o2 =>
+    match Mem.ptr2int Mem b2 0 with
+    | ret z => zeq (z + Int.signed 31 o2) (Int.unsigned 31 i1)
+    | merror => false
+    end
+| _, _ => false
+end.
+
+Fixpoint gveq Mem (gv1 gv2:GenericValue) : bool :=
+match gv1, gv2 with
+| nil, nil => true
+| (v1,c1)::gv1', (v2,c2)::gv2' => veq Mem v1 v2 && 
+                                  AST.memory_chunk_eq c1 c2 && 
+                                  gveq Mem gv1' gv2'
+| _, _ => false
+end.
+
+Lemma veq_refl : forall M v, veq M v v = true.
+Proof.
+  destruct v; simpl; auto.
+Admitted.
+
+Lemma gveq_refl : forall M gv, gveq M gv gv = true.
+Admitted.
+
+Require Import symexe_tactic.
+
+Lemma gveq__GV2val__veq : forall M gv1 gv2 TD v1, 
+  gveq M gv1 gv2 = true ->
+  GV2val TD gv1 = Some v1 ->
+  exists v2, GV2val TD gv2 = Some v2 /\ veq M v1 v2.
+Proof.
+  intros M gv1 gv2 TD v1 H1 H2.
+  unfold GV2val in H2.
+  destruct gv1; inv H2.
+  destruct p.
+  destruct gv1; inv H0.
+  simpl in H1.
+  destruct gv2; inv H1.
+  destruct p.
+  bdestruct3 H0 as H1 H2 H3.
+  destruct gv2.
+    exists v. simpl. auto.
+    inversion H3.
+Qed.
+
+Lemma alloc_ptr2int : forall z Mem0 b0 ofs0 lo hi Mem' b,
+  ret z = Mem.ptr2int Mem0 b0 ofs0 ->
+  Mem.alloc Mem0 lo hi = (Mem', b) ->
+  ret z = Mem.ptr2int Mem' b0 ofs0.
+Admitted.
+
+Lemma alloc_ptr2int' : forall Mem0 b0 ofs0 lo hi Mem' b,
+  None = Mem.ptr2int Mem0 b0 ofs0 ->
+  Mem.alloc Mem0 lo hi = (Mem', b) ->
+  (b <> b0 -> None = Mem.ptr2int Mem' b0 ofs0) \/
+  (b = b0 -> lo <= ofs0 < hi -> Some (ofs0 - lo) = Mem.ptr2int Mem' b0 ofs0) \/
+  (b = b0 -> ~ lo <= ofs0 < hi -> None = Mem.ptr2int Mem' b0 ofs0).
+Admitted.
+
+Lemma alloc__const2GV : forall lo hi Mem' b TD Mem gl c gv t, 
+  _const2GV TD Mem gl c = ret (gv,t) ->
+  Mem.alloc Mem lo hi = (Mem', b) ->
+  exists gv', _const2GV TD Mem' gl c = ret (gv',t) /\ gveq Mem' gv gv' = true.
+Proof.
+  induction c; intros; simpl in *.
+  
+  exists gv. auto using gveq_refl.
+    
+admit.
+admit.
+admit.
+admit.
+admit.
+admit.
+admit.
+admit.
+admit.
+
+(*
+  remember (_const2GV TD Mem0 gl c) as R.
+  destruct R as [[gv1 t1]|]; try solve [inversion H].
+    erewrite IHc; eauto.
+    simpl; auto.
+*)
+  remember (_const2GV TD Mem0 gl c0) as R.
+  destruct R as [[gv1 t1]|]; try solve [inversion H].
+    assert (J:=H0).
+    eapply IHc in J; eauto.
+    destruct J as [gv' [J1 J2]].
+    rewrite J1.
+    unfold mcast in *.
+    destruct c.
+(*
+      destruct t1; try solve [inversion H].
+        destruct t; try solve [inversion H]; auto.
+        destruct t; try solve [inversion H]; auto.
+*)
+      admit.
+      admit.
+      admit.
+      admit.
+
+Case "cast".
+      destruct t1; try solve [inversion H].
+      destruct t; try solve [inversion H].
+      remember (GV2val TD gv1) as R.
+      destruct R; try solve [inversion H].
+      eapply gveq__GV2val__veq in J2; eauto.          
+      destruct J2 as [v2 [J21 J22]].
+      rewrite J21.
+      destruct v; try solve [inversion H].
+        unfold veq in J22.
+        unfold is_true in J22.
+        destruct v2; try solve [inversion J22].
+            remember (Mem.ptr2int Mem0 b0 0) as R'.
+            destruct R'; inv H.
+              bdestruct J22 as J2 J3.
+              destruct (eq_block b0 b1); subst; try solve [inversion J2].
+                eapply alloc_ptr2int in HeqR'; eauto.
+                rewrite <- HeqR'.
+                exists (val2GV TD (Vint s (Int.repr s (z + Int.signed 31 i1))) (AST.Mint s)).
+                split; auto.
+                  unfold val2GV.
+                  simpl. bsplit; auto with zarith. 
+                    admit. (* zarith *)
+
+              (* vptr should take addr *)
+              admit.
+                
+            remember (Mem.ptr2int Mem0 b0 0) as R'.
+            destruct R'; inv H.
+              eapply alloc_ptr2int in HeqR'; eauto.
+              rewrite <- HeqR' in J22; try solve [inversion J22].
+              exists (val2GV TD (Vint s (Int.repr s (Int.unsigned 31 i1))) (AST.Mint s)).
+              split; auto.
+                unfold val2GV.
+                simpl. bsplit; auto with zarith.
+                  admit. (* zarith *)
+
+              (* vptr should take addr *)
+              admit.
+
+        inv H.
+        unfold veq in J22.
+        unfold is_true in J22.
+        destruct v2; try solve [inversion J22].
+            remember (Mem.ptr2int Mem' b0 0) as R'.
+            destruct R'; inv J22.
+              exists (val2GV TD (Vint s (Int.repr s (z + Int.signed 31 i1))) (AST.Mint s)).
+              split; auto.
+                  unfold val2GV.
+                  simpl.
+                    admit. (* zarith *)
+
+            exists (val2GV TD (Vint s (Int.repr s (Int.unsigned 31 i1))) (AST.Mint s)).
+            split; auto.
+                unfold val2GV.
+                simpl. 
+                  admit. (* zarith *)
+
+Case "gep".
+
+Admitted.
+
+Lemma alloc_const2GV : forall TD Mem gl c gv lo hi Mem' b, 
+  const2GV TD Mem gl c = ret gv ->
+  Mem.alloc Mem lo hi = (Mem', b) ->
+  exists gv', const2GV TD Mem' gl c = ret gv' /\ gveq Mem' gv gv' = true.
+Proof.
+  intros.
+  unfold const2GV in *.
+  remember (_const2GV TD Mem0 gl c) as R. 
+  destruct R; inv H.
+  destruct p; inv H2.
+  eapply alloc__const2GV in H0; eauto.
+  destruct H0 as [gv' [H01 H02]].
+  exists gv'. rewrite H01. auto.
+Qed.
+
 Lemma malloc_getOperandValue_inv : 
   forall Mem2 tsz gn a0 Mem2' TD v lc2 gl gv mb2,
   malloc TD Mem2 tsz gn a0 = Some (Mem2', mb2) ->
   getOperandValue TD Mem2 v lc2 gl = Some gv ->
-  getOperandValue TD Mem2' v lc2 gl = Some gv.
+  exists gv', 
+    getOperandValue TD Mem2' v lc2 gl = Some gv' /\ gveq Mem2' gv gv' = true.
 Proof.
   intros Mem2 tsz gn a0 Mem2' TD v lc2 gl gv mb2 Hmalloc Hget.
   unfold malloc in Hmalloc.
@@ -1705,10 +1910,10 @@ Proof.
   destruct R; inv Hmalloc.
   case_eq (Mem.alloc Mem2 0 (Size.to_Z tsz * z)).
   intros m b Halloc.
-  (* This could be wrong! if v is (inttoptr 42), and 42 is within the newly-
-     allocated block!. Then, Hget returns null, while the goal returns a good
-     ptr gv. *)
-Admitted. 
+  destruct v as [vid |]; simpl in *; auto.
+    exists gv. split; auto using gveq_refl.
+    eapply alloc_const2GV; eauto.
+Qed.
 
 Lemma simulation__eq__GV2int : forall mi gn gn' TD,
   gv_inject mi gn gn' ->
@@ -1721,6 +1926,27 @@ Lemma simulation__mload : forall mi TD MM Mem0 Mem2 gvp align0 gv t gvp2,
   gv_inject mi gvp gvp2 ->
   exists gv2, mload TD Mem2 gvp2 t align0 = ret gv2 /\ gv_inject mi gv gv2.
 Admitted.
+
+Lemma gveq__eq__GV2int : forall Mem gn gn' TD,
+  gveq Mem gn gn' ->
+  GV2int TD Size.ThirtyTwo gn = GV2int TD Size.ThirtyTwo gn'.
+Proof.
+  intros.
+  unfold GV2int.
+  destruct gn.
+    destruct gn'; auto.
+      simpl in H. unfold is_true in H. inv H.
+    destruct gn'.
+      simpl in H. destruct p. unfold is_true in H. inv H.
+      simpl in H. destruct p. destruct p0.
+      bdestruct3 H as H1 H2 H3.
+      destruct v; destruct v0; try solve [auto | inversion H1].
+        destruct gn; destruct gn'; try solve [auto | inversion H3].
+          admit.    
+          simpl in H3. destruct p. inversion H3.
+        admit. (* H1 shoule be false *)
+        admit. (* H1 shoule be false *)
+Qed.
 
 Lemma trans_cmd__is__correct__dbMalloc : forall 
   (lc2 : GVMap)
@@ -1832,13 +2058,16 @@ Proof.
       (Mem2:=Mem2'); auto.
 
       assert (exists gn', getOperandValue TD Mem2' v lc2 gl = ret gn' /\
-                          gv_inject mi gn gn') as H4.
+              GV2int TD Size.ThirtyTwo gn = GV2int TD Size.ThirtyTwo gn') as H4.
         eapply simulation__getOperandValue with (MM:=MM)(Mem2:=Mem2) in H0
           ; eauto.
         destruct H0 as [gv' [H00 H01]].
         apply malloc_getOperandValue_inv with (tsz:=tsz)(gn:=gn)(a0:=align0)
          (Mem2':=Mem2')(mb2:=mb') in H00; auto.
-        exists gv'. auto.
+        destruct H00 as [gv'' [H0a H0b]].
+        exists gv''. split; auto.
+          rewrite simulation__eq__GV2int with (mi:=mi)(gn':=gv'); eauto.
+          eapply gveq__eq__GV2int; eauto.
       destruct H4 as [gn' [H41 H42]].
       apply SimpleSE.dbGEP with (mp:=blk2GV TD mb')(vidxs:=[gn']); auto.
         simpl.
@@ -1857,8 +2086,7 @@ Proof.
 
         unfold SoftBound.bound2GV, GEP, blk2GV, GV2ptr, ptr2GV, val2GV.
         simpl.
-        erewrite simulation__eq__GV2int in H2; eauto.
-        rewrite H2.
+        rewrite <- H42. rewrite H2.
         unfold mgetoffset. destruct TD.
         unfold typ2utyp. simpl.
         assert (exists ut, typ2utyp_aux (gen_utyp_maps (rev n0)) t = Some ut)
